theories/coneris/examples/hash/con_hash_interface4.v
@@ -8,7 +8,122 @@ Set Default Proof Using "Type*".
  *)
 
 
+Class con_hash4 `{!conerisGS Σ} (val_size max_key : nat ):= Con_Hash4
+{
+  (** * Operations *)
+  init_con_hash : val;
+  compute_con_hash : val;
+  (** * Ghost state *)
 
+  (** [name] is used to associate [locked] with [is_lock] *)
+  (* tape_name: Type; *)
+
+  (** * Predicates *)
+  conhashfun (γs : gname * gname) (f : val) : iProp Σ;
+  hashkey (γs : gname * gname) (k : nat) (v : option nat) : iProp Σ;
+
+  (** * General properties of the predicates *)
+  (* #[global] concrete_seq_hash_timeless {L : seq_hashG Σ} f m :: *)
+  (*   Timeless (concrete_seq_hash (L:=L) f m); *)
+  #[global] hashkey_timeless γs k v ::
+    Timeless (hashkey γs k v);
+  #[global] conhashfun_persistent γs f ::
+    Persistent (conhashfun γs f);
+  #[global] hashkey_Some_persistent γs k v ::
+  Persistent (hashkey γs k (Some v));
+  hashkey_exclusive γs k v v' ::
+    hashkey γs k v -∗ hashkey γs k v'  -∗ False;
+  hash_key_valid γs k v n :
+    hashkey γs k v -∗ ⌜ v = Some n ⌝ -∗ ⌜ (n ≤ val_size)%nat ⌝;
+
+  hashkey_presample E k (bad : gset nat) (ε εI εO: nonnegreal) γs :
+  (* Note: there should be no way for you to own a hashkey for
+     a key out of range, so this is redundant
+    k ≤ max_key →
+  *)
+    (∀ x, x ∈ bad → x < S val_size) →
+    (εI * size bad + εO * (val_size + 1 - size bad) <= ε * (val_size + 1))%R →
+    hashkey γs k None -∗
+    ↯ ε -∗
+    state_update E E (∃ (n : fin (S val_size)),
+        ((⌜fin_to_nat n ∉ bad⌝ ∗ ↯ εO) ∨ (⌜fin_to_nat n ∈ bad⌝ ∗ ↯ εI)) ∗
+          hashkey γs k (Some (fin_to_nat n)));
+
+  conhash_init :
+  {{{ True }}}
+    init_con_hash #()
+  {{{ (γs : gname * gname) conhash, RET conhash;
+        conhashfun γs conhash ∗
+        ([∗ set] k ∈ (set_seq 0 (S max_key)), hashkey γs k None)  }}} ;
+
+  wp_conhashfun_prev f (k n : nat) γs :
+  {{{ conhashfun γs f ∗ hashkey γs k (Some n) }}}
+    f #k
+  {{{ RET #n; conhashfun γs f ∗ hashkey γs k (Some n) }}}
+
+}.
+
+
+Section derived_lemmas.
+  Context `{conerisGS Σ, !con_hash4 val_size max_key}.
+
+Lemma wp_hash_lookup_safe k f γs :
+    {{{ hashkey γs k None ∗ conhashfun γs f }}}
+        f #k
+    {{{ (v : nat), RET #v; ⌜ (v ≤ val_size)%nat ⌝ ∗ hashkey γs k (Some v) ∗ conhashfun γs f }}}.
+  Proof.
+    iIntros (Φ) "(HNone & #Hinv) HΦ".
+    iMod (ec_zero) as "Herr".
+    iApply state_update_pgl_wp.
+    iMod (hashkey_presample _ _ ∅ nnreal_zero nnreal_zero nnreal_zero with "HNone [Herr]")
+        as "(%v & _ & Hhauth)"; auto.
+      + set_solver.
+      + rewrite size_empty /=.
+        lra.
+      + iModIntro.
+        wp_apply (wp_conhashfun_prev with "[-HΦ]"); auto.
+        iIntros "(?&?)".
+        iApply "HΦ".
+        iFrame.
+        iPureIntro.
+        pose proof (fin_to_nat_lt v).
+        lia.
+   Qed.
+
+
+Lemma wp_hash_lookup_avoid_set k f γs (bad : gset nat)(ε εI εO:nonnegreal) :
+    (forall x : nat, x ∈ bad -> (x < S val_size)%nat) ->
+    (εI * (size bad) + εO * (val_size + 1 - size bad) <= ε * (val_size + 1))%R ->
+    {{{ ↯ ε ∗ hashkey γs k None ∗ conhashfun γs f }}}
+      f #k
+      {{{ (v : nat), RET #v; ⌜ (v ≤ val_size)%nat ⌝ ∗
+                             ((⌜v ∈ bad⌝) ∗ ↯ εI  ∨
+                                (⌜v ∉ bad⌝) ∗ ↯ εO) ∗
+                             hashkey γs k (Some v) }}}.
+  Proof.
+    iIntros (Hbad Hdistr Φ) "(Herr & Hnone & #Hinv) HΦ".
+    iApply state_update_pgl_wp.
+    iMod (hashkey_presample _ _ bad ε εI εO with "Hnone [Herr]")
+      as "(%v & Hv & Hhauth)"; auto.
+    iModIntro.
+    wp_apply (wp_conhashfun_prev with "[-HΦ Hv]"); auto.
+    iIntros "(?&?)".
+    iApply "HΦ".
+    iFrame.
+    iSplit.
+    {
+      iPureIntro.
+      pose proof (fin_to_nat_lt v).
+      lia.
+    }
+    iDestruct "Hv" as "[?|?]"; auto.
+  Qed.
+
+End derived_lemmas.
+
+(*
+
+Old interface
 
 Class con_hash4 `{!conerisGS Σ} (val_size max_key : nat ):= Con_Hash4
 {
@@ -153,3 +268,4 @@ Section derived_lemmas.
 
 End derived_lemmas.
 
+*)
